proofs/itrees/it_sems_core_proofs.v
@@ -22,7 +22,7 @@ From ITree Require Import
      ITree
      ITreeFacts
      Monad
-     Basics.HeterogeneousRelations     
+     Basics.HeterogeneousRelations
      Events.Map
      Events.State
      Events.StateFacts
@@ -55,11 +55,11 @@ From ITree Require Import
      Interp.InterpFacts
      Interp.Recursion.
 
-From ITree Require Import Rutt RuttFacts.
+From ITree Require Import XRutt XRuttFacts.
 
 From ITree Require Import EqAxiom.
 
-From Jasmin Require Import expr psem_defs psem oseq.
+From Jasmin Require Import expr psem_defs psem oseq compiler_util xrutt_aux.
 From Jasmin Require Import it_gen_lib it_jasmin_lib it_sems_core.
 
 Import Monads.
@@ -73,8 +73,6 @@ Unset Strict Implicit.
 Unset Printing Implicit Defensive.
 *)
 
-Obligation Tactic := done || idtac.
-
 (* PROBLEM with sections *)
 
 (* This files contains proofs to test the semantic models in
@@ -84,30 +82,100 @@ Obligation Tactic := done || idtac.
  need to be revised. The proofs on the flat models are much longer and
  more laden with detail than those on the error-aware model. *)
 
-Section Lang.
-Context (asm_op: Type) (asmop: asmOp asm_op).
+Class with_Error (E: Type -> Type) {HasErr: ErrEvent -< E} := {
+  is_error : forall {X}, E X -> bool;
+  is_error_has : forall {X} (e:ErrEvent X) , is_error (HasErr X e)
+}.
+Arguments with_Error : clear implicits.
+Arguments with_Error E {_}.
 
+Definition ErrorCutoff {E: Type -> Type} {HasErr: ErrEvent -< E} {wE : with_Error E} X (m : E X) :=
+  ~~(is_error m).
+
+Definition NoCutoff {E: Type -> Type} {HasErr: ErrEvent -< E} {wE : with_Error E} X (m : E X) := true.
+
+Definition rutt_err {E1 E2: Type -> Type}
+  {HasErr1: ErrEvent -< E1} {wE1 : with_Error E1}
+  {HasErr2: ErrEvent -< E2} {wE2 : with_Error E2}
+  {O1 O2 : Type}
+  (pre_event : prerel E1 E2)
+  (post_event: postrel E1 E2)
+  (post      : O1 -> O2 -> Prop) :=
+  @rutt E1 E2 O1 O2 ErrorCutoff NoCutoff pre_event post_event post.
+
+Instance with_Errorr_suml {E: Type -> Type} {HasErr: ErrEvent -< E} {wE : with_Error E} (T:Type -> Type) :
+  with_Error (T +' E).
+Proof.
+  apply (@Build_with_Error _ _  (fun X s => match s with | inr1 e => is_error e | _ => false end)).
+  move=> x e => /=.
+  apply is_error_has.
+Qed.
+
+(*
+Existing Instance HasErr.
+ *)
+(*
+
+
+
+Section CUTOFF.
+
+
+
+Context (E: Type -> Type).
+Context (HasErr: ErrEvent -< E).
+
+Context (E0: Type -> Type).
+Context (FI: FIso (E0 +' ErrEvent) E).
+
+Definition ErrorCutoff X (m : E X) :=
+  match mfun2 _ m with
+  | inl1 _ => true
+  | inr1 x => false
+  end.
+
+Definition NoCutoff : forall X, E X -> bool :=
+  fun X m => true.
+
+End CUTOFF.
+
+*)
 Section WSW.
-Context {wsw: WithSubWord}.   
 Context
-  (dc: DirectCall)
-  (syscall_state : Type)
-  (ep : EstateParams syscall_state)
-  (spp : SemPexprParams)
-  (sip : SemInstrParams asm_op syscall_state)
-  (pT : progT)
-  (scP : semCallParams)
+  {asm_op: Type}
+  {asmop: asmOp asm_op}
+  {wsw: WithSubWord}
+  {dc: DirectCall}
+  {syscall_state : Type}
+  {ep : EstateParams syscall_state}
+  {spp : SemPexprParams}
+  {sip : SemInstrParams asm_op syscall_state}
+  {pT : progT}
+  {scP : semCallParams}
   (ev : extra_val_t).
 
-Local Notation FunE := (FunE asmop).
-Local Notation FFCall_ := (FFCall asmop). 
-Local Notation cmd_Ind := (cmd_Ind asm_op asmop).
-Local Notation FunDef := (FunDef asmop pT).
-Local Notation FCState := (FCState asmop ep).
-Local Notation meval_instr := (meval_instr spp scP). 
-Local Notation meval_fcall := (meval_fcall dc spp scP ev). 
-Local Notation mevalE_cmd := (mevalE_cmd dc spp scP ev). 
+Section Section.
 
+  Context {E1 E2: Type -> Type}
+          {HasErr1 : ErrEvent -< E1} {HasErr2 : ErrEvent -< E2}
+          {wE1 : with_Error E1} {wE2 : with_Error E2}
+        (TR_E : forall T1 T2,
+            E1 T1 -> E2 T2 -> Prop)
+        (VR_E : forall T1 T2,
+            E1 T1 -> T1 -> E2 T2 -> T2 -> Prop).
+
+Lemma rutt_iresult (T1 T2:Type) st1 st2 (x1 : exec T1) (x2 : exec T2) (R : T1 -> T2 -> Prop) :
+  (forall v1, x1 = ok v1 -> exists2 v2, x2 = ok v2 & R v1 v2) ->
+  rutt_err TR_E VR_E R (iresult st1 x1) (iresult st2 x2).
+Proof.
+  case: x1 => [ v1 | e1] hok.
+  + have [v2 -> /=] := hok _ erefl.
+    by apply: rutt_Ret.
+  apply rutt_CutL => //.
+  by rewrite /ErrorCutoff /= is_error_has.
+Qed.
+
+End Section.
 
 (***************************************************************************)
 (*** APPLICATION ***********************************************************)
@@ -126,7 +194,7 @@ Local Notation tr_lvals ls := (map tr_lval ls).
 Local Notation tr_exprs es := (map tr_expr es).
 
 Definition Tr_i (Th: instr_r -> instr_r) (i: instr) : instr :=
-  match i with MkI ii ir => MkI ii (Th ir) end.  
+  match i with MkI ii ir => MkI ii (Th ir) end.
 
 Fixpoint Tr_ir (i : instr_r) : instr_r :=
   let R := Tr_i Tr_ir in
@@ -137,122 +205,132 @@ Fixpoint Tr_ir (i : instr_r) : instr_r :=
   | Csyscall xs sc es =>
       Csyscall (tr_lvals xs) (tr_sysc sc) (tr_exprs es)
   | Cif e c1 c2 => Cif (tr_expr e) (map R c1) (map R c2)
-  | Cfor i rg c => Cfor i rg (map R c)                     
+  | Cfor i rg c => Cfor i rg (map R c)
   | Cwhile a c1 e c2 => Cwhile a (map R c1) (tr_expr e) (map R c2)
   | Ccall xs fn es => Ccall (tr_lvals xs) fn (tr_exprs es)
   end.
+
 Local Notation Tr_instr := (Tr_i Tr_ir).
 Local Notation Tr_cmd c := (map Tr_instr c).
 
-Definition Tr_FunDef (f: FunDef) : FunDef :=
+Definition Tr_FunDef (f: fundef) : fundef :=
   match f with
   | MkFun i tyin p_xs c tyout r_xs xtr =>
     MkFun i tyin p_xs (Tr_cmd c) tyout r_xs xtr end.
-    
 
 (*********************************************************************)
 (*** PROOFS **********************************************************)
 
 Section TR_tests.
 
-Context (pr1 pr2 : prog)
-        (PR : forall T, T -> T -> Prop).
-Context (TR_E : forall (E: Type -> Type) T1 T2,
+Context (pr1 : prog).
+
+Let pr2 := map_prog Tr_FunDef pr1.
+
+Context (E: Type -> Type)
+        (TR_E : forall T1 T2,
             E T1 -> E T2 -> Prop)
-        (VR_E : forall (E: Type -> Type) T1 T2,
+        (VR_E : forall T1 T2,
             E T1 -> T1 -> E T2 -> T2 -> Prop).
 
-Local Notation RS := (PR estate).
+
+
+
+(*Local Notation RS := (PR estate).
 Local Notation RV := (PR values).
 Local Notation RV1 := (PR value).
 Local Notation RSMV := (PR (syscall_state * mem * seq value)).
+*)
 
+Context (FI: FIso (void1 +' ErrEvent) E).
 
-Section GEN_ErrAndFlat.
-
-Context (E: Type -> Type).   
-
-Local Notation RV := (PR values).
+(*
 Local Notation VS := (values * estate)%type.
 Local Notation FVS := (funname * VS)%type.
 
-Notation RVS := (fun (vs_st1 vs_st2 : VS) => 
+Notation RVS := (fun (vs_st1 vs_st2 : VS) =>
   (RV vs_st1.1 vs_st2.1 /\ RS vs_st1.2 vs_st2.2)).
-Notation RFVS := (fun (fvs1 fvs2 : FVS) => 
+Notation RFVS := (fun (fvs1 fvs2 : FVS) =>
   (fvs1.1 = fvs2.1 /\ RVS fvs1.2 fvs2.2)).
 Notation RC := (fun c1 c2: cmd => c2 = Tr_cmd c1).
 Notation RFunDef := (fun f1 f2: FunDef => f2 = Tr_FunDef f1).
+
 
 Context (rvs_def : PR VS = RVS)
         (rfvs_def : PR FVS = RFVS)
         (rc_def : PR cmd = RC)
         (rfundef_def : PR FunDef = RFunDef).
 
+*)
 
-Section GEN_Error.
+Context (HasErr: ErrEvent -< E).
+Context (wE: with_Error E).
 
-Context (HasErr: ErrState -< E).   
+Definition RC c1 c2 := Tr_cmd c1 = c2.
+
+Context
+   (Rv  : value -> value -> Prop)
+   (Rscs: syscall_state_t -> syscall_state_t -> Prop)
+   (Rm  : mem -> mem -> Prop)
+   (RS  : estate -> estate -> Prop).
+
+Notation Rvs := (List.Forall2 Rv).
+
+Definition Rfres (fres1 fres2 : syscall_state_t * mem * values) :=
+   [/\ Rscs fres1.1.1 fres2.1.1
+      , Rm fres1.1.2 fres2.1.2
+      & Rvs fres1.2 fres2.2].
 
 Section TR_MutualRec.
 
 (* ME: relation between FCState events *)
 Definition TR_D_ME {T1 T2} (d1 : FCState T1)
                            (d2 : FCState T2) : Prop :=
-  match (d1, d2) with
-  | (FLCode c1 st1, FLCode c2 st2) => RC c1 c2 /\ RS st1 st2
-  | (FFCall xs1 fn1 es1 st1, FFCall xs2 fn2 es2 st2) =>
-      xs2 = map tr_lval xs1 /\ fn1 = fn2 /\ es2 = map tr_expr es1 /\ RS st1 st2
-  | _ => False   
-  end.               
+  match d1, d2 with
+  | FLCode c1 st1, FLCode c2 st2 => RC c1 c2 /\ RS st1 st2
+  | FFCall scs1 m1 fn1 vs1, FFCall scs2 m2 fn2 vs2 =>
+    [/\ Rscs scs1 scs2
+      , Rm m1 m2
+      , fn1 = fn2
+      & Rvs vs1 vs2]
+  | _, _ => False
+  end.
 
 (* ME: relation between FCState event outputs, i.e. over estate *)
-Program Definition VR_D_ME {T1 T2}
-  (d1 : FCState T1) (t1: T1) (d2 : FCState T2) (t2: T2) : Prop.
-  dependent destruction d1.
-  - dependent destruction d2.
-    + exact (RS t1 t2).
-    + exact (False).
-  - dependent destruction d2.
-    + exact (False).
-    + exact (RS t1 t2).     
-Defined.      
-
-(* NOT USED *)
-(*
-Definition FCState_det {T} (d: FCState T) : T = estate :=
- match d in (it_sems_core.FCState _ _ T0) return (T0 = estate) with
- | FLCode c st => (fun=> (fun=> erefl)) c st
- | @FFCall _ _ _ _ _ xs f es st =>
-     (fun=> (fun=> (fun=> (fun=> erefl)))) xs f es st
- end.
-Definition st_cast {T} (d: FCState T) (x: T) : estate.
-  rewrite (FCState_det d) in x; exact x.
-Defined.
-Definition VR_D_ME' {T1 T2}
+Definition VR_D_ME {T1 T2}
   (d1 : FCState T1) (t1: T1) (d2 : FCState T2) (t2: T2) : Prop :=
-  (match (d1, d2) return (estate -> estate -> Prop) with
-  | (FLCode c1 st1, FLCode c2 st2) => RS 
-  | (FFCall xs1 f1 es1 st1, FFCall xs2 f2 es2 st2) => RS 
-  | _ => fun _ _ => False end)
-    (st_cast d1 t1) (st_cast d2 t2).
-*)
+  match d1 in FCState T1_ return T1_ -> T2 -> Prop with
+  | FLCode _ _ =>
+    match d2 in FCState T2_ return estate -> T2_ -> Prop with
+    | FLCode _ _ => RS
+    | FFCall _ _ _ _ => fun _ _ => False
+    end
+  | FFCall _ _ _ _ =>
+    match d2 in FCState T2_ return syscall_state_t * mem * values -> T2_ -> Prop with
+    | FLCode _ _ => fun _ _ => False
+    | FFCall _ _ _ _ => Rfres
+    end
+  end t1 t2.
+
 (***)
 
-Program Definition TR_DE_ME : prerel (FCState +' E) (FCState +' E) :=
-  sum_prerel (@TR_D_ME) (TR_E E).
+Program Definition TR_DE : prerel (FCState +' E) (FCState +' E) :=
+  sum_prerel (@TR_D_ME) TR_E.
 
-Program Definition VR_DE_ME : postrel (FCState +' E) (FCState +' E) :=
-  sum_postrel (@VR_D_ME) (VR_E E).
+Program Definition VR_DE : postrel (FCState +' E) (FCState +' E) :=
+  sum_postrel (@VR_D_ME) VR_E.
 
+(*
 Context (fcstate_t_def : TR_E (FCState +' E) = TR_DE_ME).
 Context (fcstate_v_def : VR_E (FCState +' E) = VR_DE_ME).
-
-Lemma rutt_err_eval_Args fn es1 st1 st2 : 
+*)
+(*
+Lemma rutt_err_eval_Args fn es1 st1 st2 :
   RS st1 st2 ->
   rutt (TR_E (FCState +' E)) (VR_E (FCState +' E)) RV
     (err_eval_Args dc spp pr1 fn es1 st1)
     (err_eval_Args dc spp pr2 fn (tr_exprs es1) st2).
-Admitted. 
+Admitted.
 
 Lemma rutt_err_init_state fn r1 r2 st1 st2 :
   RV r1 r2 ->
@@ -260,92 +338,140 @@ Lemma rutt_err_init_state fn r1 r2 st1 st2 :
   rutt (TR_E (FCState +' E)) (VR_E (FCState +' E)) RS
     (err_init_state dc scP ev pr1 fn r1 st1)
     (err_init_state dc scP ev pr2 fn r2 st2).
-Admitted.   
+Admitted.
 
 Lemma rutt_err_get_FunCode fn :
   rutt (TR_E (FCState +' E)) (VR_E (FCState +' E)) RC
     (err_get_FunCode pr1 fn)
-    (err_get_FunCode pr2 fn).    
-Admitted. 
+    (err_get_FunCode pr2 fn).
+Admitted.
 
 Lemma rutt_err_return_val fn st1 st2 :
   RS st1 st2 ->
   rutt (TR_E (FCState +' E)) (VR_E (FCState +' E)) RV
     (err_return_val dc pr1 fn st1)
-    (err_return_val dc pr2 fn st2).    
-Admitted. 
+    (err_return_val dc pr2 fn st2).
+Admitted.
 
 Lemma rutt_err_reinstate_caller fn xs v1 v2 st1 st2 st3 st4 :
   RV v1 v2 ->
   RS st1 st2 ->
   RS st3 st4 ->
   rutt (TR_E (FCState +' E)) (VR_E (FCState +' E))
-    RS   
+    RS
     (err_reinstate_caller dc spp scP pr1 fn xs v1
        st1 st3)
     (err_reinstate_caller dc spp scP pr2 fn
        (tr_lvals xs) v2 st2 st4).
-Admitted. 
-
+Admitted.
+*)
 (***)
 
-Lemma rutt_err_mk_AssgnE x tg ty e st1 st2 :
-  RS st1 st2 ->
-  rutt (sum_prerel (@TR_D_ME) (TR_E E)) (sum_postrel (@VR_D_ME) (VR_E E)) RS
-    (err_mk_AssgnE spp pr1 x tg ty e st1)
-    (err_mk_AssgnE spp pr2 (tr_lval x) tg ty (tr_expr e) st2).
-Admitted.   
+Check @rutt.
 
-Lemma rutt_err_mk_OpnE x tg o e st1 st2 :
+Lemma rutt_err_assgn x tg ty e st1 st2 :
   RS st1 st2 ->
-  rutt (sum_prerel (@TR_D_ME) (TR_E E)) (sum_postrel (@VR_D_ME) (VR_E E)) RS
-    (err_mk_OpnE spp pr1 x tg o e st1)
-    (err_mk_OpnE spp pr2 (tr_lvals x) tg (tr_opn o) (tr_exprs e) st2).
-Admitted. 
+  rutt_err TR_DE VR_DE RS
+    (iresult st1 (eval_assgn pr1 x tg ty e st1))
+    (iresult st2 (eval_assgn pr2 (tr_lval x) tg ty (tr_expr e) st2)).
+Proof.
+  move=> hrs; apply rutt_iresult.
+Admitted.
 
+Lemma rutt_err_opn x o e st1 st2 :
+  RS st1 st2 ->
+  rutt_err TR_DE VR_DE RS
+    (iresult st1 (sem_sopn (p_globs pr1) o st1 x e))
+    (iresult st2 (sem_sopn (p_globs pr2) o st2 (tr_lvals x) (tr_exprs e))).
+Admitted.
+
+
+Lemma rutt_cmd_tr_ME_step (i: instr_r) (st1 st2: estate) :
+  RS st1 st2 ->
+  rutt_err TR_DE VR_DE RS (msem_i pr1 i st1) (msem_i pr2 (Tr_ir i) st2).
+Proof.
+  case: i.
+  + by move=> x tag ty e hst /=; apply rutt_err_assgn.
+  + admit.
+  + admit.
+  + move=> e c1 c2 hst /=.
+    apply rutt_bind with (RR := eq).
+    + admit.
+    move=> b _ <-.
+    apply rutt_trigger => /=.
+    + by apply sum_prerel_inl => /=; split => //; case: b.
+    move=> t1 t2; rewrite /VR_DE.
+
+ econstructor.
+apply sum_postrel_inl.
+
+
+Search sum_prerel.
+ /sum_prerel /=.
+
+
+
+
+Set Printing All.
+
+
+nstr
+
+
+    (sum_prerel (@TR_D_ME) (TR_E E))
+    (sum_postrel (@VR_D_ME) (VR_E E))
+    RS (st_cmd_map_r (meval_instr pr1) cc st1)
+    (st_cmd_map_r (meval_instr pr2) (Tr_cmd cc) st2).
+
+(*
 Lemma rutt_err_mk_SyscallE x sc e st1 st2 :
   RS st1 st2 ->
   rutt (sum_prerel (@TR_D_ME) (TR_E E)) (sum_postrel (@VR_D_ME) (VR_E E)) RS
     (err_mk_SyscallE spp scP pr1 x sc e st1)
-    (err_mk_SyscallE spp scP pr2 
+    (err_mk_SyscallE spp scP pr2
        (tr_lvals x) (tr_sysc sc) (tr_exprs e) st2).
-Admitted. 
+Admitted.
 
 Lemma rutt_err_mk_EvalCond e st1 st2 :
   RS st1 st2 ->
    rutt (sum_prerel (@TR_D_ME) (TR_E E)) (sum_postrel (@VR_D_ME) (VR_E E)) eq
     (err_mk_EvalCond spp pr1 e st1)
     (err_mk_EvalCond spp pr2 (tr_expr e) st2).
-Admitted.  
+Admitted.
 
 Lemma rutt_err_mk_EvalBound e st1 st2 :
   RS st1 st2 ->
   rutt (sum_prerel (@TR_D_ME) (TR_E E)) (sum_postrel (@VR_D_ME) (VR_E E)) eq
     (err_mk_EvalBound spp pr1 e st1)
     (err_mk_EvalBound spp pr2 e st2).
-Admitted. 
+Admitted.
 
 Lemma rutt_err_mk_WriteIndex xi z st1 st2 :
   RS st1 st2 ->
    rutt (sum_prerel (@TR_D_ME) (TR_E E)) (sum_postrel (@VR_D_ME) (VR_E E)) RS
     (err_mk_WriteIndex xi z st1) (err_mk_WriteIndex xi z st2).
-Admitted. 
-
+Admitted.
+*)
+(*
 Lemma comp_gen_ok_ME (fn: funname)
   (xs1 xs2: lvals) (es1 es2: pexprs) (st1 st2: estate) :
   xs2 = map tr_lval xs1 ->
-  es2 = map tr_expr es1 -> 
+  es2 = map tr_expr es1 ->
   RS st1 st2 ->
-  @rutt (FCState +' E) _ _ _ (TR_E _) (VR_E _)
+  rutt_err TR_DE VR_DE
+   (msem_i
+
+
+ (FCState +' E) _ _ _ (TR_E _) (VR_E _)
     (fun a1 a2 => @VR_D_ME _ _ (FFCall_ xs1 fn es1 st1) a1
-                             (FFCall_ xs2 fn es2 st2) a2)  
+                             (FFCall_ xs2 fn es2 st2) a2)
     (meval_fcall pr1 xs1 fn es1 st1) (meval_fcall pr2 xs2 fn es2 st2).
   intros.
   unfold meval_fcall; simpl.
-  
+
   eapply rutt_bind with (RR := RV); inv H; intros.
 
-  { eapply rutt_err_eval_Args; auto. }    
+  { eapply rutt_err_eval_Args; auto. }
 
   eapply rutt_bind with (RR := RS); intros.
 
@@ -357,12 +483,12 @@ Lemma comp_gen_ok_ME (fn: funname)
 
   inv H2. eapply rutt_bind with (RR := RS); intros.
   { eapply rutt_trigger; simpl; intros.
-    { rewrite fcstate_t_def. 
+    { rewrite fcstate_t_def.
       econstructor.
       split; auto; intros.
     }
     rewrite fcstate_v_def in H2.
-    dependent destruction H2.    
+    dependent destruction H2.
     unfold VR_D_ME in H2; auto.
   }
 
@@ -370,43 +496,43 @@ Lemma comp_gen_ok_ME (fn: funname)
   { eapply rutt_err_return_val; auto. }
 
   assert ((fun a1 : estate => [eta RS a1]) = RS) as A1.
-  { eauto. } 
-  
+  { eauto. }
+
   rewrite A1; eapply rutt_err_reinstate_caller; auto.
 Qed.
-
+*)
 (* Inductive lemma - GOOD. here we are not tying the coinductive knot,
    as st_cmd_map_r is just a map function. *)
-Lemma rutt_cmd_tr_ME_step (cc: cmd) (st1 st2: estate) : 
+Lemma rutt_cmd_tr_ME_step (cc: cmd) (st1 st2: estate) :
   RS st1 st2 ->
-  @rutt (FCState +' E) _ _ _
+  rutt_err (FCState +' E) _ _ _
     (sum_prerel (@TR_D_ME) (TR_E E))
     (sum_postrel (@VR_D_ME) (VR_E E))
     RS (st_cmd_map_r (meval_instr pr1) cc st1)
     (st_cmd_map_r (meval_instr pr2) (Tr_cmd cc) st2).
   simpl; intros.
 
-  set (Pr := fun (i: instr_r) => forall ii st1 st2, RS st1 st2 -> 
+  set (Pr := fun (i: instr_r) => forall ii st1 st2, RS st1 st2 ->
      @rutt (FCState +' E) _ _ _
     (sum_prerel (@TR_D_ME) (TR_E E))
     (sum_postrel (@VR_D_ME) (VR_E E))
-    RS 
+    RS
     (st_cmd_map_r (meval_instr pr1) ((MkI ii i) :: nil) st1)
     (st_cmd_map_r (meval_instr pr2) ((Tr_instr (MkI ii i)) :: nil) st2)).
 
-  set (Pi := fun (i: instr) => forall st1 st2, RS st1 st2 -> 
+  set (Pi := fun (i: instr) => forall st1 st2, RS st1 st2 ->
      @rutt (FCState +' E) _ _ _
     (sum_prerel (@TR_D_ME) (TR_E E))
     (sum_postrel (@VR_D_ME) (VR_E E))
-    RS 
+    RS
     (st_cmd_map_r (meval_instr pr1) (i :: nil) st1)
     (st_cmd_map_r (meval_instr pr2) ((Tr_instr i) :: nil) st2)).
 
-  set (Pc := fun (c: cmd) => forall st1 st2, RS st1 st2 -> 
+  set (Pc := fun (c: cmd) => forall st1 st2, RS st1 st2 ->
      @rutt (FCState +' E) _ _ _
     (sum_prerel (@TR_D_ME) (TR_E E))
     (sum_postrel (@VR_D_ME) (VR_E E))
-    RS 
+    RS
     (st_cmd_map_r (meval_instr pr1) c st1)
     (st_cmd_map_r (meval_instr pr2) (Tr_cmd c) st2)).
 
@@ -424,10 +550,10 @@ Lemma rutt_cmd_tr_ME_step (cc: cmd) (st1 st2: estate) :
   }
 
   { eapply rutt_bind with (RR := RS); intros.
-    eapply rutt_err_mk_AssgnE; auto.     
-    eapply rutt_Ret; eauto. 
+    eapply rutt_err_mk_AssgnE; auto.
+    eapply rutt_Ret; eauto.
   }
-    
+
   { eapply rutt_bind with (RR := RS); intros.
     eapply rutt_err_mk_OpnE; auto.
     eapply rutt_Ret; eauto.
@@ -441,16 +567,16 @@ Lemma rutt_cmd_tr_ME_step (cc: cmd) (st1 st2: estate) :
   { intros.
     eapply rutt_bind with (RR := RS); intros.
     { eapply rutt_bind with (RR := eq); intros.
-      { eapply rutt_err_mk_EvalCond; auto. } 
+      { eapply rutt_err_mk_EvalCond; auto. }
       inv H2; destruct r2; simpl.
       eapply H; eauto.
       eapply H0; eauto.
-    }  
+    }
     eapply rutt_Ret; auto.
   }
 
   { eapply rutt_bind with (RR := RS); simpl; intros.
-    destruct rn; destruct p; simpl.    
+    destruct rn; destruct p; simpl.
     eapply rutt_bind with (RR := eq); simpl; intros.
     eapply rutt_err_mk_EvalBound; auto.
 
@@ -461,13 +587,13 @@ Lemma rutt_cmd_tr_ME_step (cc: cmd) (st1 st2: estate) :
     induction (wrange d r2 r0); simpl; intros.
     { eapply rutt_Ret; eauto. }
     { eapply rutt_bind with (RR:= RS); simpl; intros.
-      { eapply rutt_err_mk_WriteIndex; auto. } 
+      { eapply rutt_err_mk_WriteIndex; auto. }
       eapply rutt_bind with (RR := RS); intros; auto.
     }
-      
+
     eapply rutt_Ret; auto.
   }
-    
+
   { eapply rutt_bind with (RR := RS); intros.
     eapply rutt_iter with (RI := RS); intros; auto.
     eapply rutt_bind with (RR := RS); intros.
@@ -482,30 +608,30 @@ Lemma rutt_cmd_tr_ME_step (cc: cmd) (st1 st2: estate) :
     eapply rutt_Ret; auto.
     eapply rutt_Ret; auto.
     eapply rutt_Ret; auto.
-  }   
-    
+  }
+
   { eapply rutt_bind with (RR := RS); intros.
     eapply rutt_trigger; simpl; intros.
     econstructor.
     unfold TR_D_ME; simpl.
     split; eauto.
 
-    simpl in H0.     
-    
+    simpl in H0.
+
     intros; auto.
     simpl in H0.
     dependent destruction H0; auto.
     eapply rutt_Ret; auto.
-  }  
+  }
 Qed.
 
 (* Here we apply the inductive lemma and comp_gen_ok *)
-Lemma rutt_cmd_tr_ME (cc: cmd) (st1 st2: estate) : 
+Lemma rutt_cmd_tr_ME (cc: cmd) (st1 st2: estate) :
   RS st1 st2 ->
-  @rutt E _ _ _ 
+  @rutt E _ _ _
     (TR_E _) (VR_E _) RS
     (mevalE_cmd pr1 cc st1) (mevalE_cmd pr2 (Tr_cmd cc) st2).
-Proof.  
+Proof.
   intros; unfold mevalE_cmd; simpl.
   eapply interp_mrec_rutt; simpl; intros.
   { instantiate (3 := @TR_D_ME).
@@ -516,18 +642,18 @@ Proof.
       destruct d2; try intuition.
       inv H1; simpl.
       eapply rutt_cmd_tr_ME_step; eauto.
-    }  
-   
+    }
+
     { unfold TR_D_ME in H0.
       destruct d2; simpl in *; try intuition.
-      inv H0.  
+      inv H0.
       have CC := (comp_gen_ok_ME f0 xs _ es _ _ _ erefl erefl H4).
       setoid_rewrite fcstate_t_def in CC.
       setoid_rewrite fcstate_v_def in CC.
       eapply CC.
-    }  
-  }         
-  eapply rutt_cmd_tr_ME_step; eauto. 
+    }
+  }
+  eapply rutt_cmd_tr_ME_step; eauto.
 Qed.
 
 
